Add case for App

soundness.v
@@ -4,7 +4,7 @@ From Hammer Require Import Tactics.
 
 
 Definition γ_ok n Γ γ := forall i, i < n -> forall PA, InterpType (subst_tm γ (dep_ith Γ i)) PA -> PA (γ i).
-Definition SemWt n Γ a A := forall γ, γ_ok n Γ γ -> exists PA, InterpType (subst_tm γ A) PA /\ PA a.
+Definition SemWt n Γ a A := forall γ, γ_ok n Γ γ -> exists PA, InterpType (subst_tm γ A) PA /\ PA (subst_tm γ a).
 Definition SemUWf n Γ A := forall γ, γ_ok n Γ γ -> exists PA, InterpType (subst_tm γ A) PA.
 
 Theorem soundness n Γ a A (h : Wt n Γ a A) : SemWt n Γ a A.
@@ -18,6 +18,22 @@ Proof.
   - hauto l:on.
   - admit.
   - admit.
-  - admit.
+  - move => n Γ f A B b _ ihf _ ihb γ hγ.
+    rewrite /SemWt in ihf ihb.
+    move /(_ γ hγ) : ihf; intros (PPi & hPi & hf).
+    move /(_ γ hγ) : ihb; intros (PA & hPA & hb).
+    simpl in hPi.
+    move /InterpType_Fun_inv' : hPi;
+      intros (PA0 & PF & hPA0 & hPFTot & hPF & ?); subst.
+    have ? : forall x, PA x <-> PA0 x by eauto using InterpType_deterministic.
+    have hPA0b : PA0 (subst_tm γ b) by sfirstorder.
+    move /(_ _ hPA0b) : hPFTot; intros (PB & hPB).
+    have hPB' := hPF _ PB hPA0b hPB.
+    move /(_ _ PB hPA0b hPB) in hPF.
+    rewrite /ProdSpace in hf.
+    asimpl in *.
+    exists PB; split; first done.
+    move /(_ _ hPA0b) : hf; intros (PB0 & hPB0 & hPB0').
+
   - admit.
 Admitted.
